第一题：
$$
\begin{align}
解:\\
&先证明两个常用结论:\\
&\neg p\Lrarr\neg (p\vee p)\Lrarr p\darr p\\
&\neg p\Lrarr\neg (p\wedge p)\Lrarr p\uarr p\\
(1)\\
&\neg p\vee q\\
&\Lrarr\neg\neg(\neg p\vee q)\\
&\Lrarr\neg(\neg p\darr q)\\
&\Lrarr\neg((p\darr p)\darr q)\\
&\Lrarr((p\darr p)\darr q)\darr((p\darr p)\darr q)\\\\
&\neg p\vee q\\
&\Lrarr\neg p\vee\neg\neg q\\
&\Lrarr\neg(p\wedge\neg q)\\
&\Lrarr p\uarr\neg q\\
&\Lrarr p\uarr(q\uarr q)\\
(2)\\
&p\wedge\neg q\\
&\Lrarr \neg\neg p\wedge\neg q\\
&\Lrarr\neg(\neg p\vee q)\\
&\Lrarr \neg p\darr q\\
&\Lrarr (p\darr p)\darr q\\\\
&p\wedge\neg q\\
&\Lrarr\neg\neg(p\wedge\neg q)\\
&\Lrarr\neg(p\uarr\neg q)\\
&\Lrarr\neg(p\uarr(q\uarr q))\\
&\Lrarr(p\uarr(q\uarr q))\uarr(p\uarr(q\uarr q))\\
(3)\\
&\neg p\vee\neg q\\
&\Lrarr\neg\neg(\neg p\vee\neg q)\\
&\Lrarr\neg(\neg p\darr\neg q)\\
&\Lrarr\neg((p\darr p)\darr(q\darr q))\\
&\Lrarr((p\darr p)\darr(q\darr q))\darr((p\darr p)\darr(q\darr q))\\\\
&\neg p\vee\neg q\\
&\Lrarr\neg(p\wedge q)\\
&\Lrarr p\uarr q\\
(4)\\
& p \lrarr q \\
&\Lrarr (p \wedge q) \vee (\neg p \wedge \neg q) \\
&\Lrarr \neg(\neg p \vee \neg q)\vee\neg(p\vee q)\\
&\Lrarr(\neg p\darr\neg q)\vee(p\darr q)\\
&\Lrarr((p\darr p)\darr(q\darr q))\vee(p\darr q)\\
&\Lrarr\neg\neg(((p\darr p)\darr(q\darr q))\vee(p\darr q))\\
&\Lrarr\neg(((p\darr p)\darr(q\darr q))\darr(p\darr q))\\
&\Lrarr(((p\darr p)\darr(q\darr q))\darr(p\darr q))\darr(((p\darr p)\darr(q\darr q))\darr(p\darr q))\\\\
&p\lrarr q\\
&\Lrarr (p \wedge q) \vee (\neg p \wedge \neg q) \\
&\Lrarr\neg(\neg(p\wedge q)\wedge\neg(\neg p\wedge\neg q))\\
&\Lrarr\neg((p\uarr q)\wedge(\neg p\uarr\neg q))\\
&\Lrarr(p\uarr q)\uarr(\neg p\uarr\neg q)\\
&\Lrarr(p\uarr q)\uarr((p\uarr p)\uarr(q\uarr q))\\
\end{align}
$$
第二题：

$$
\begin{align}
2.~&解:\\
(1&)\\
&a.~\neg A\rarr(A\rarr B)~~~定理6\\
&b.~(A\rarr B)\rarr(A\rarr B)~~~定理1\\
&c.~(A\rarr(A\rarr B))\rarr(A\rarr B)~~~a和b用定理18\\
(3&)\\
&a.~\neg(B\rarr C)\rarr\neg A~~~已知定理\\
&b.~(\neg(B\rarr C)\rarr\neg A)\rarr(A\rarr(B\rarr C))~~~公理3\\
&c.~A\rarr(B\rarr C)~~~a与c用分离规则\\
&d.~(A\rarr(B\rarr C))\rarr((A\rarr B)\rarr(A\rarr C))~~~公理2\\
&e.(A\rarr B)\rarr(A\rarr C)~~~c与d用分离规则\\
&f.A\rarr B~~~已知定理\\
&g.A\rarr C~~~e与f用分离规则\\
(5&)\\
&a.~(C\rarr D)\rarr((B\rarr C)\rarr(B\rarr D))~~~定理4\\
&b.~((B\rarr C)\rarr(B\rarr D))\rarr((A\rarr(B\rarr C))\rarr(A\rarr(B\rarr D)))~~~定理4\\
&c.~(C\rarr D)\rarr((A\rarr(B\rarr C))\rarr(A\rarr(B\rarr D)))~~~a和b用三段论定理8\\
&d.~(A\rarr(B\rarr C))\rarr((C\rarr D)\rarr(A\rarr(B\rarr D)))~~~对c用前件互换定理2\\
(7&)\\
&a.~\neg A\rarr(A\rarr B)~~~定理6\\
&b.~(\neg A\rarr(A\rarr B))\rarr(\neg(A\rarr B)\rarr A)~~~定理14\\
&c.~\neg(A\rarr B)\rarr A~~~a和b用分离规则\\
&d.~A\rarr(B\rarr A)~~~公理1\\
&e.~\neg(A\rarr B)\rarr(B\rarr A)~~~c和d用三段论定理8\\
&f.~(B\rarr A)\rarr(B\rarr A)~~~定理1\\
&g.((A\rarr B)\rarr(B\rarr A))\rarr(B\rarr A)~~~e和f用定理18\\
(9&)\\
&a.~\neg A\rarr(A\rarr B)~~~定理6\\
&b.~(\neg A\rarr(A\rarr B))\rarr(\neg(A\rarr B)\rarr A)~~~定理14\\
&c.~\neg(A\rarr B)\rarr A~~~a与b用分离规则\\
&d.~A\rarr A~~~定理1\\
&e.((A\rarr B)\rarr A)\rarr A~~~c和d用定理18\\
(11&)\\
&a.~\neg A\rarr(A\rarr B)~~~定理6\\
&b.~(\neg A\rarr(A\rarr B))\rarr(((A\rarr B)\rarr C)\rarr(\neg A\rarr C))~~~定理5\\
&c.~((A\rarr B)\rarr C)\rarr(\neg A\rarr C)~~~a和b用分离规则\\
&d.~(\neg A\rarr C)\rarr(\neg C\rarr A)~~~定理14\\
&e.~((A\rarr B)\rarr C)\rarr(\neg C\rarr A)~~~c和d用三段论定理8\\
&f.~(\neg C\rarr A)\rarr((A\rarr C)\rarr(\neg C\rarr C))~~~定理5\\
&g.~((A\rarr B)\rarr C)\rarr((A\rarr C)\rarr(\neg C\rarr C))~~~e和f用三段论定理8\\
&h.~(\neg C\rarr C)\rarr C~~~定理9\\
&i.~((\neg C\rarr C)\rarr C)\rarr(((A\rarr C)\rarr(\neg C\rarr C))\rarr ((A\rarr C)\rarr C))~~~定理4\\
&j.~((A\rarr C)\rarr(\neg C\rarr C))\rarr((A\rarr C)\rarr C)~~~h和i用分离规则\\
&k.~((A\rarr B)\rarr C)\rarr((A\rarr C)\rarr C)~~~g和j用三段论定理8\\
(13&)\\
&a.~\neg A\rarr(A\rarr B)~~~定理6\\
&b.~(\neg A\rarr(A\rarr B))\rarr(((A\rarr B)\rarr B)\rarr(\neg A\rarr B))~~~定理5\\
&c.~((A\rarr B)\rarr B)\rarr(\neg A\rarr B)~~~a和b用分离规则\\
&d.~((A\rarr B)\rarr B)\rarr(\neg A\rarr B))\rarr
	\\&~~~~~~~~~~~~~~~~~(((\neg A\rarr B)\rarr C)\rarr(((A\rarr B)\rarr B)\rarr C))~~~定理5\\
&e.~((\neg A\rarr B)\rarr C)\rarr(((A\rarr B)\rarr B)\rarr C)~~~c和d用分离规则\\
&f.~((\neg A\rarr B)\rarr C)\rarr(((A\rarr B)\rarr B)\rarr C)\rarr\\
	&~~(((B\rarr C)\rarr((\neg A\rarr B)\rarr C))\rarr((B\rarr C)\rarr(((A\rarr B)\rarr B)\rarr C)))~~~定理4\\
&g.~((B\rarr C)\rarr((\neg A\rarr B)\rarr C))\rarr\\
	&~~~~~~~~~~~~~~~~((B\rarr C)\rarr(((A\rarr B)\rarr B)\rarr C))~~~e和f用分离规则\\
&h.~(A\rarr C)\rarr((B\rarr C)\rarr((\neg A\rarr B)\rarr C))~~~定理22\\
&i.~(A\rarr C)\rarr((B\rarr C)\rarr(((A\rarr B)\rarr B)\rarr C))~~~g和h用三段论定理8
\end{align}
$$

