1.1
$$
\begin{align}
&(1).B\rarr A~~~~假设\\
&(2).\neg A~~~~假设\\
&(3).(B\rarr A)\rarr(\neg A\rarr\neg B)~~~~定理13\\
&(4).\neg A\rarr\neg B~~~~(1)和(3)用分离规则\\
&(5).\neg B~~~~(2)和(4)用分离规则\\
&(6).B\rarr A,\neg A\vdash\neg B~~~~演绎结果的定义\\
&(7).B\rarr A\vdash\neg A\rarr\neg B~~~~演绎定理\\
&(8).\vdash(B\rarr A)\rarr(\neg A\rarr\neg B)~~~~演绎定理
\end{align}
$$
1.2
$$
\begin{align}
&(1).A\rarr B~~~~假设\\
&(2).B\rarr C~~~~假设\\
&(3).A~~~~假设\\
&(4).B~~~~(1)和(3)用分离规则\\
&(5).C~~~~(2)和(4)用分离规则\\
&(6).A\rarr B,B\rarr C,A\vdash C~~~~演绎结果的定义\\
&(7).A\rarr B,B\rarr C\vdash A\rarr C~~~~演绎定理\\
&(8).A\rarr B\vdash(B\rarr C)\rarr(A\rarr C)~~~~演绎定理\\
&(9).\vdash(A\rarr B)\rarr((B\rarr C)\rarr(A\rarr C))~~~~演绎定理\\
\end{align}
$$
1.3
$$
\begin{align}
&(1).(A\rarr B)\rarr A~~~~假设\\
&(2).\neg A\rarr A~~~~(1)用定理18\\
&(3).(\neg A\rarr A)\rarr A~~~~定理9\\
&(4).A~~~~(2)和(3)用分离规则\\
&(5).(A\rarr B)\rarr A\vdash A~~~~演绎结果的定义\\
&(6).\vdash((A\rarr B)\rarr A)\rarr A~~~~演绎定理\\
\end{align}
$$


1.4
$$
\begin{align}
&(1).\neg (A\rarr B)~~~~假设\\
&(2).B~~~~假设\\
&(3).\neg A\rarr(A\rarr B)~~~~定理6\\
&(4).(\neg A\rarr(A\rarr B))\rarr(\neg(A\rarr B)\rarr A)~~~~定理14\\
&(5).\neg(A\rarr B)\rarr A~~~~(3)和(4)用分离规则\\
&(6).A~~~~(1)和(5)用演绎定理\\
&(7).\neg (A\rarr B), B\vdash A~~~~演绎结果的定义\\
&(8).\neg (A\rarr B)\vdash B\rarr A~~~~演绎定理\\
&(9).\vdash\neg (A\rarr B)\rarr(B\rarr A)~~~~演绎定理\\
\end{align}
$$




2.1
$$
\begin{align}
&(1).\neg\neg A\rarr A~~~~定理10\\
&(2).A\rarr((\neg A\rarr\neg B)\rarr A)~~~~公理1\\
&(3).\neg\neg A\rarr((\neg A\rarr\neg B)\rarr A)~~~~(1)和(3)用三段论定理8\\
&(4).(\neg A\rarr\neg B)\rarr(B\rarr A)~~~~公理3\\
&(5).B\rarr((\neg A\rarr\neg B)\rarr A)~~~~(4)用前件互换定理2\\
&(6).(\neg A\rarr B)\rarr((\neg A\rarr\neg B)\rarr A)~~~~(3)和(5)用定理18\\
\end{align}
$$
2.2
$$
\begin{align}
&().~~~~\\
&().~~~~\\
&().~~~~\\
&().~~~~\\
&().~~~~\\
&().~~~~\\
&().~~~~\\
&().~~~~\\
&().~~~~\\
&().~~~~\\
&().~~~~\\
&().~~~~\\
&().~~~~\\
&().~~~~\\
&().~~~~\\
\end{align}
$$




